\documentclass[handout]{beamer}
%\documentclass[slides]{beamer}
% Vary the color applet  (try out your own if you like)
%\colorlet{structure}{red!20!black}
%\beamertemplateshadingbackground{yellow!20}{white}
%\usepackage{beamerthemeshadow}
%\usepackage[utf8x]{inputenc} CONFLICT!
\usepackage{tikz}
%\usepackage[english,norsk,nynorsk]{babel}
\usepackage{tikz-cd}
\usetikzlibrary{trees}

\usepackage[all]{xy}
\usepackage{multicol}

%\setbeamertemplate{navigation symbols}{}++++++
%\setbeamertemplate{footline}[frame number]
\usetheme{Montpellier}


\input macros

\newcommand{\To}{\Rightarrow}
\newcommand{\Trt}{\stackrel{*}{\Rightarrow}}
\newcommand{\ToG}{\Rightarrow_G}
\newcommand{\redS}{{\color{red} S}}

\newcommand{\bfsf}[1]{{\boldsymbol{#1}}}
\newcommand{\Set}{\bfsf{Set}}
\newcommand{\Gra}{\bfsf{Graph}}
\newcommand{\CC}{\bfsf{C}}
\newcommand{\DD}{\bfsf{D}}
\newcommand{\EE}{\bfsf{E}}
\newcommand{\PP}{\bfsf{P}}
\newcommand{\HH}{\bfsf{H}}
\newcommand{\Nat}{\bfsf{Nat}}
\newcommand{\Incl}{\bfsf{Incl}}
\newcommand{\Rel}{\bfsf{Rel}}
\newcommand{\Mult}{\bfsf{Mult}}
\newcommand{\Mon}{\bfsf{Mon}}
\newcommand{\Cat}{\bfsf{Cat}}
\newcommand{\CAT}{\bfsf{CAT}}

\newcommand{\Kp}[1]{{\langle #1 \rangle}}
\newcommand{\Kc}{;\!;}
\newcommand{\bind}{{>}\!\!{>}\!{=}}
\newcommand{\ttt}[1]{\text{\tt #1}}

\title[INF223 presentations]{}

\begin{document}

\section{Monads}
\subsection{Introduction}
 
\frame
  {   
    \frametitle{Monads}\label{Mon5:Intro}

 \begin{itemize}[<+->]
\item Monads were defined in CT in the (late) 1950's and 1960's and  
turned out to be useful in programming
\item A breakthrough paper for application in CS was 
\href{https://person.dibris.unige.it/moggi-eugenio/ftp/ic91.pdf}{\color{blue}E. Moggi, Notions of computation and monads, I\&C, 93(1), 1991}
\item Idea: a computation can be more than a function from input 
of type $A$ to output of type $B$ (side-effects, exceptions, etc.)
\item We start by giving two examples, and then carefully abstract from 
these to arrive at the (equivalent) notion(s) of a monad
\item Useful links are:
 \begin{itemize}
    \item \myurl{https://ncatlab.org/nlab/show/monad+\%28in+computer+science\%29}
    \item \myurl{https://ncatlab.org/nlab/show/extension+system}
 \end{itemize}
 \end{itemize}

 }

\frame
  {   
    \frametitle{A reinterpretation of multimaps}\label{Mon5:MultiMapReint}

 \begin{itemize}[<+->]
\item Recall $\Mult$ with sets as objects and morphisms $f:A\to B$ being
\emph{multimaps}, that is, set maps $f: A\to \powset(B)$
\item Recall the power set functor $\Set\to\Set$ mapping sets to their power set
and $f:A\to B$  to $\powset(f) : \powset(A) \to \powset(B)$ defined by $\powset(f)(X) = f(X)$, the {\color{red}image} of any given $X\subseteq A$
\item We reformulate the composition of $f:A\to \powset(B)$ and $g:B\to \powset(C)$
in three steps:
 \begin{enumerate}
    \item form $\powset(g) : \powset(B) \to \powset(\powset(C))$
    \item take the ordinary composition $f;\powset(g) : A \to \powset(\powset(C))$
    \item finish by `flattening' , i.e., by postcomposing with 
$\mu_C:$ $\powset(\powset(C)) \to \powset(C) $ defined by 
$\mu_C(X) = \bigcup X$ for all $X\subseteq\powset(C)$
 \end{enumerate}
We obtain the same composition of $f$ and $g$ in $\Mult$ as in the script, Def. 2.3.30.
Proof on next slide:
 \end{itemize}

 }

\frame
  {   
    \frametitle{A reinterpretation of multimaps (cntd)}\label{Mon5:MultiMapReint}

 \begin{itemize}[<+->]
\item For any $a\in A$ we have $f(a)\subseteq B$ and {\color{red}image}
$g(f(a)) =$ $ \set{g(y) \mid y\in f(a)}$. Each $g(y)$ is a subset of $C$.
Applying $\mu_C$ gives $\bigcup \set{g(y) \mid y\in f(a)}$, formula (2.11)
in the script.
\item Also useful: $\eta_A: A \to \powset(A)$ by $\eta_A(a)=\set{a}$
\item Together, $\Set, \powset, \eta, \mu$ form the ingredients of a monad
\item Some properties, later introduced as the monad laws: 
 \begin{enumerate}
\item $\powset(\eta_A)(X) = \set{\set{x}\mid x\in X}$,
the {\color{red}image} of $X$ under $\eta_A$, and $\eta_{\powset(A)}(X) = \set{X}$,
for any $X\subseteq A$. Their $\mu_A$ values, i.e., $\bigcup$, are $X$ for both!
So: $\mu_A(\powset(\eta_A)(X)) = \mu_A(\eta_{\powset(A)}(X)) = X$.
% for all $X\subseteq A$.
\item For $X\subseteq \powset^2(A)$, the {\color{red}image} 
$\mu_A(X) = \set{\mu_A(Y)\mid Y\in X}$
and $\mu_{\powset(A)}(X)=\bigcup X$. Applying $\mu_A$ gives in both cases
$\set{a\in A \mid \linebreak \exists Z,Y~a\in Z\in Y \in X}$. 
So: 
$\mu_A(\powset(\mu_A)(X)) = \mu_A(\mu_{\powset(A)}(X))$.
 \end{enumerate}
\item Exercise: find $X=\set{Y_1,Y_2}$ with 
$\bigcup X \neq \set{\bigcup Y_1, \bigcup Y_2}$.
Show point 2 above, i.e., $\bigcup(\bigcup X) = \bigcup \set{\bigcup Y \mid Y\in X}$
 \end{itemize}

 }

\frame
  {   
    \frametitle{Another example of a monad: the Writer}\label{Mon5:ExaSetMone}

 \begin{itemize}[<+->]
\item In Haskell this is the 
\href{https://wiki.haskell.org/All_About_Monads\#The_Writer\_monad}%
{\color{blue}Writer} monad
\item We work in the category $\Set$ and fix a monoid $(M,1,*)$
\item This example models functions that write a string as side-effect
(strings with the empty string and concatenation form a monoid)
\item Operation $T$ on sets is defined by $T(X)= X\times M$
\item Map $f : X\to Y$ with side-effect $p : X\to M$ is modelled as $\Kp{f,p} : X\to T(Y)$
%$p$ gives the monoid value as a side-effect of $f$
\item For every set $X$ we define $unit_X: X\to T(X)$ mapping $x\in X$ to $(x,1)$,
so $unit_X = \Kp{id_X,x\mapsto 1}$
\item For the moment $unit_X$ is just an example, but it will turn out to
be some kind of neutral element
 \end{itemize}
 }

\frame
  {   
    \frametitle{Another example of a monad: the Writer (ctnd)}\label{Mon5:ExaSetMctnd}

 \begin{itemize}[<+->]
\item For $\Kp{f,p}: X\to T(Y)$ and $\Kp{g,q}: Y\to T(Z)$ we define a special
composition $\Kp{f,p}\Kc \Kp{g,q} = \Kp{f;g,r} : X\to T(Z)$ with $$r(x)=p(x)*q(f(x))$$
Thus the monoid-valued-side-effect is cumulative,
we multiply the old value $p(x)$ by the new value $q(f(x))$,
or, we append the string $q(f(x))$ to the string $p(x)$.
\item Indeed we get an identity law: for $\Kp{f,p}: X\to T(Y)$ we have
$$unit_X\Kc \Kp{f,p}  = \Kp{f,p} = \Kp{f,p}\Kc unit_Y$$
\item Also, the special composition $\Kc$ is associative  (exercise)
\item Note that the left and right unit are (subtly) different.
We don't have a new \emph{monoid}, but we do have a \emph{monad}.
 \end{itemize}

 }

\frame
  {   
    \frametitle{Categorical abstraction from the Writer (one)}\label{Mon5:CatAbstrOne}

 \begin{itemize}[<+->]
\item For $\Kp{f,p} : X\to T(Y)$ we define $\Kp{f,p}^T : T(X)\to T(Y)$ by
$$\Kp{f,p}^T(x,v) = (f(x),v*p(x))$$
\item Exercise: show $\Kp{f,p}\Kc\Kp{g,q} = \Kp{f,p};\Kp{g,q}^T$
\item Preparing for abstraction from the example,
we extend $T$ to a functor $\Set\to\Set$ 
by setting, for any $f:X\to Y$,  $$T(f) = (f; unit_Y)^T : T(X)\to T(Y)$$
\item In evidence: $T(f) = f\times id_M$ and, as required for a functor,
\begin{itemize}
\item
$T(id_X) = id_X \times id_M = id_{X\times M} = id_{T(X)}$  for all $X$
\item $T(f;g) = (f;g)\times id_M = (f\times id_M);(g\times id_M) = T(f); T(g)$
for all $f:X\to Y$ and $g:Y\to Z$
\end{itemize}
 \end{itemize}

 }

\frame
  {   
    \frametitle{Categorical abstraction from the Writer (two)}\label{Mon5:CatAbstrTwo}

 \begin{itemize}[<+->]
\item With $T$ a functor the family $unit_X: X\to T(X)$ appears to be
a natural transformation $id_\Set \To T$, with naturality square:
%\varepsilon:
\[
\begin{tikzcd}[ampersand replacement=\&]
X \arrow[swap]{d}{f} \& X  \arrow[swap]{d}{f}\arrow{r}{unit_X} \&\arrow{d}{T(f)} T(X)\\
Y \& Y  \arrow{r}{unit_Y} \& T(Y)
\end{tikzcd}
\]
$(f;unit_Y)(x)=(f(x),1) = T(f)(x,1) = (unit_X;T(f))(x)$
\item We want to get the special composition right (cf.\ multimaps)
\item Maps $\Kp{f,p}: X\to T(Y)$ and $\Kp{g,q}: Y\to T(Z)$ cannot be composed
in $\Set$, but $T(\Kp{g,q}) : T(Y) \to T(T(Z))$ gives the composite
$$\Kp{f,p};T(\Kp{g,q}) : X \to T(T(Z))$$
\item Not there yet: the latter type should be $X \to T(Z)$
 \end{itemize}

 }


\frame
  {
    \frametitle{Categorical abstraction (three)}\label{Mon5:CatAbstrThree}

 \begin{itemize}[<+->]
\item Note $T(\Kp{g,q})(y,w) =  (\Kp{g,q}(y),w) = ((g(y),q(y)),w)$, so
$(\Kp{f,p};T(\Kp{g,q}))(x) = (g(f(x)),q(f(x))),p(x)): T(T(Z))$
\item Recall: $(\Kp{f,p}\Kc \Kp{g,q})(x) = (g(f(x)),p(x)*q(f(x)) : T(Z)$
\item The missing step from $T(T(Z))$ to $T(Z)$ is taken by
$$\mu_Z: T(T(Z))\to T(Z): ((z,m_{new}),m_{old}) \mapsto (z,m_{old}*m_{new})$$
and $\mu$ is a natural transformation, the \emph{monad multiplication}:
\[
\begin{tikzcd}[ampersand replacement=\&]
X \arrow[swap]{d}{f} \& T(T(X))  \arrow[swap]{d}{T(T(f))}\arrow{r}{\mu_X} \&\arrow{d}{T(f)} T(X)\\
Y \& T(T(Y))  \arrow{r}{\mu_Y} \& T(Y)
\end{tikzcd}
\]
since $\mu_Y(T(T(f))((x,m'),m)) = \mu_Y((f(x),m'),m) = (f(x), m*m')
= T(f)(x,m*m') = T(f)(\mu_X((x,m'),m))$
 \end{itemize}

 }

\frame
  {   
    \frametitle{Picture of the two ways of composing}\label{Mon5:PicTwoMonad}

% \begin{itemize}[<+->]
%\item The CT way (left) and the CS way (right)

\begin{tikzcd}[ampersand replacement=\&]
\&\& T(T(C))\arrow{d}{\mu_C} \&
\\
\& T(B)\arrow{ur}{T(g)}\& T(C) \&
\& T(B)\arrow{r}{g^T}\& T(C)\\
A\arrow{ur}{f}\arrow[dashed,swap]{urr}[description]{f;;g}\&B\arrow[swap]{ur}{g}\& \&
A\arrow{ur}{f}\arrow[dashed,swap]{urr}[description]{f;;g}\&B\arrow[swap]{ur}{g}\&
\end{tikzcd}

\vspace*{1em}
Left is common in Category Theory, right in Computer Science

 %\end{itemize}

 }


\frame
  {   
    \frametitle{A categorical definition of monad}\label{Mon5:CatDefMonad}

 \begin{itemize}[<+->]
\item A \emph{monad} consists of the following data:
 \begin{enumerate}
    \item a category $\CC$
    \item a functor $T:\CC\to\CC$
    \item a natural transformation $\eta: id_\CC \To T$ (the \emph{monad unit})
    \item a natural transformation $\mu: T;T \To T$ (the \emph{multiplication})
 \end{enumerate}
satisfying the following properties:
 \begin{enumerate}
    \item $\eta_{T(A)};\mu_A = id_{T(A)} = T(\eta_A);\mu_A$ (the \emph{monad identity} laws)
    \item $T(\mu_A);\mu_A = \mu_{T(A)};\mu_A$ (the \emph{monad associativity} law)
 \end{enumerate}
\item Exercise: verify that all equalities above are well-typed
\item We carefully review the examples from the previous slides to 
make sure that they were indeed monads. 
The terms \emph{monad unit, multiplication} etc.\ will be explained.
 \end{itemize}

 }

\frame
  {   
    \frametitle{Revisiting the power set monad}\label{Mon5:PowSetMonad}

 \begin{itemize}[<+->]
\item The \emph{power set monad} consists of the following data:
 \begin{enumerate}
    \item the category $\Set$
    \item the functor $\powset:\Set\to\Set$, NB $\powset(f)(X) = f(X)$, the {\color{red}image}
    \item the natural transformation $\eta: id_\Set \To T$, $\eta_A(a)=\set{a}$
    \item the natural transformation $\mu$, 
$\mu_A: \powset(\powset(A)) \to \powset(A) $ defined by 
$\mu_A(X) = \bigcup X$ for all $X\subseteq\powset(A)$
 \end{enumerate}
\item The naturality squares commute (exercise, NB $\powset^2(f)$!):
\begin{tikzcd}[ampersand replacement=\&]
A \arrow[swap]{d}{f} \& 
A  \arrow[swap]{d}{f}\arrow{r}{\eta_A} \&\arrow{d}{\powset(f)} \powset(A)\&
\powset^2(A)\arrow[swap]{d}{\powset^2(f)}\arrow{r}{\mu_A} \&\arrow{d}{\powset(f)} \powset(A)\\
B \& 
B  \arrow{r}{\eta_B} \& \powset(B) \&
\powset^2(B)\arrow{r}{\mu_B} \& \powset(B)
\end{tikzcd}
\item The monad laws hold (last two points on slide \ref{Mon5:MultiMapReint}):
 \begin{enumerate}
    \item $\eta_{\powset(A)};\mu_A = id_{\powset(A)} = \powset(\eta_A);\mu_A$
    \item $\powset(\mu_A);\mu_A = \mu_{\powset(A)};\mu_A$
 \end{enumerate}
 \end{itemize}

 }

\frame
  {   
    \frametitle{The action of the power set functor on a map}\label{Mon5:PowSetActMap}

 \begin{itemize}[<+->]
\item $\powset(f)$ applied to $X\subseteq A$ returns the {\color{red}image}
$f(X)$, the set with $f$ applied to all elements of $X$
(any order, duplicates ignored)
\item $\powset(f)$ pushes $f$ inside the outer curly brackets of its argument
\item This is much like $map\, f$ applied to a list $\ell$, returning a list with $f$ 
applied to all elements of $\ell$ (same order, duplicates possible)

\item $\powset(f)(\set{\ldots,a,\ldots}) = \set{\ldots,f(a),\ldots}$ 
%($f$ applied to all elements)
\item Iterating this for $\powset(\powset(f))$ we get:
 \end{itemize}
$$\begin{array}{rcl}\powset^2(f)(\set{\ldots,\set{\ldots,a,\ldots},\ldots})& = &
 \set{\ldots,\powset(f)(\set{\ldots,a,\ldots}),\ldots}\\
& = & 
 \set{\ldots,\set{\ldots,f(a),\ldots},\ldots}\end{array}$$

Now it should be easier to see that $\eta:id_\Set\To\powset$ and
$\mu:\powset;\powset\To\powset$ are natural transformations.
Note that $f$ could be constant. Ignoring duplicates is easiest
(idempotency rules!).
 }
\frame
  {   
    \frametitle{Some informal explanations}\label{Mon5:InfoMonad}

 \begin{itemize}[<+->]
\item One view on a monad $(\CC,T,\eta,\mu)$ is that the objects $T(A)$ are $A$
with some structure added, detailed by $\eta,\mu$. The following explanation
makes only sense for some categories $\CC$, such as $\Set$ and $\HH$ 
(sets/types + functions).
\item $T(A)$ can be viewed as the set/type of $A$-values with {\color{red}extras (!)}
\item $\eta_A : A\to T(A)$ adds a neutral extra, say 1, to any $A$-value
\item $\eta_{T(A)} : T(A)\to T^2(A)$ adds this 1 to any $T(A)$-value $(a,e)$
\item $\mu_A: T^2(A)\to T(A)$ {\color{red}combines (!)} two extras into one
\item $\eta_{T(A)};\mu_A = id_{T(A)}$ means $\mu_A((a,e),1) = (a,e)$, cf.\ $e*1=e$
\item For $f:A\to B$ the `natural' $T(f)$ maps $(a,e)$ to $(f(a),e)$
\item Hence $T(\eta_A) : T(A)\to T^2(A)$ maps $(a,e)$ to $((a,1),e)$
\item $T(\eta_A);\mu_A=id_{T(A)}$ means $\mu_A((a,1),e) = (a,e)$, cf.\ $1*e=e$
\item $T(\mu_A);\mu_A = \mu_{T(A)};\mu_A$ cf.\ $(e*e')*e'' = e*(e'*e'')$
 \end{itemize}

 }


\frame
  {   
    \frametitle{The Writer is indeed a monad (one)}\label{Mon5:ExaMonad}

 \begin{itemize}[<+->]
\item The data in the example was: the category $\Set$, 
the functor $T:\Set\to\Set$ on slide \ref{Mon5:CatAbstrOne}, 
the natural transformation $\eta: id_\Set\To T$
defined by $\eta_X = unit_X$ on slide \ref{Mon5:CatAbstrTwo}, 
the natural transformation $\mu: T;T \To T$
on slide \ref{Mon5:CatAbstrThree}. Proofs of properties:
\item $\eta_{T(A)};\mu_A = id_{T(A)}$ means that  $(\eta_{T(A)};\mu_A)(a,m) = (a,m)$
for all $a\in A, m\in M$. Indeed $\mu_A(\eta_{T(A)}(a,m)) = \mu_A((a,m),1) =$ $= (a,1*m) = (a,m)$
by the left identity law in the monoid $M$
\item Exercise: verify  $id_{T(A)} = T(\eta_A);\mu_A$ using $T(f) = f\times id_M$
\item $T(\mu_A);\mu_A = \mu_{T(A)};\mu_A$ means that the two functions agree
on all $(a,m,m',m'')$ (flat notation). $T(\mu_A)$ and $\mu_{T(A)}$ give images $(a,m'*m,m'')$ and $(a,m,m''*m')$. Thereafter $\mu_A$ gives $(a,m''*(m'*m))$ and $(a,(m''*m')*m)$, which are equal by associativity in the monoid $M$.
 \end{itemize}

 }

\frame
  {   
    \frametitle{The auxiliaries of Writer are definable in any monad}\label{Mon5:ExaMonadAux}

 \begin{itemize}[<+->]
\item We must also check that $\_^T, \Kc$ can be defined using $T,\eta,\mu$
 \begin{itemize}
\item the \emph{extension} $f^T = T(f);\mu_Y$ for all $f: X\to T(Y)$\footnote{Abstractly, here and below,
we use $f$ instead of $\Kp{f,p}:X\to T(Y)$}
\item $f \Kc  g = f ;T(g);\mu_Z$ for all $f: X\to T(Y)$, $g: Y\to T(Z)$
 \end{itemize}
\item The latter $\Kc$ is called \emph{Kleisli} composition, and is proved
associative, by using monad structure and properties only:\\
if also $h: Z\to T(A)$, then
$(f \Kc g) \Kc h = (f ;T(g);\mu_Z) \Kc h = f ;T(g);(\mu_Z; T(h)) ; \mu_A =
f ;T(g);(T^2(h);\mu_{T(A)}) ; \mu_A$ by naturality (exercise: draw the naturality diagram). 
Also, $f \Kc (g \Kc h) = f \Kc (g;T(h);\mu_A) = f; T(g;T(h);\mu_A);\mu_A =
f; T(g);T^2(h);(T(\mu_A);\mu_A) = f; T(g);T^2(h);(\mu_{T(A)};\mu_A)$
by functoriality and the \emph{monad associativity} law.

\item Exercise: verify all the steps in these proofs
 \end{itemize}

 }

\frame
  {   
    \frametitle{Monads in Haskell}\label{Mon5:MonadHask}

 \begin{itemize}[<+->]
\item $\HH$ is the \emph{syntactic category} of Haskell (types + functions)
\item The type of $\_^T$ is $(X\to T(Y)) \to (T(X)\to T(Y))$
\item In Haskell the arguments are swapped to obtain:
$$\bind : T(X) \to (X\to T(Y)) \to T(Y)~~\text{(pronounced \emph{bind}})$$
\item Interpretation: given $m:T(X)$ and $f: X\to T(Y)$, %to compute $(m\bind f):T(Y)$,
bind the argument of $f$ to the $X$-value $x$ of $m$ and compute $f(x)$;
the $T(Y)$-value of $m\bind f$ is the $Y$-value of $f(x):T(Y)$ and
the extra of $m\bind f$ is the {\color{red}combination} of 
the extras of $m$ and $f(x)$. The latter is the `magic' of the monad in question.
\item $\eta_X$ is called \ttt{return} in Haskell (a kind of misnomer),
the type subscript is left out as it can be inferred


 \end{itemize}

 }

\frame
  {   
    \frametitle{Monads in Haskell (ctnd)}\label{Mon5:MonadHaskCtnd}

 \begin{itemize}[<+->]
\item The monad laws now take the following (equivalent) form:
\begin{enumerate}
    \item $((\ttt{return}\,a)\, \bind f) = f(a)$ (left unit law)
    \item $(m\, \bind \ttt{return}) = m$ (right unit law)
    \item $(m\, \bind f) \bind g = (m\, \bind \lambda x. (f(x) \bind g))$ (associativity)
 \end{enumerate}
\item $\mu_A$ is definable by $\mu_A(m) = (m\bind id_{T(A)})$ for all $m\in T(T(A))$
(verify type and explain)
%\item The monad properties (laws) from slide \ref{Mon5:CatDefMonad} can be proved
\item Exercise (big, not difficult): prove the equivalence of the monad laws in Haskell 
and in CT (slide \ref{Mon5:CatDefMonad})
\item Haskell provides syntactic support for monads through the type class
\href{https://wiki.haskell.org/All_About_Monads}%
{\color{blue}\ttt{Monad}}, but the truth of the monad laws (the compiler expects them to hold)
is your own responsibility
 \end{itemize}

 }


\frame
  {   
    \frametitle{The list monad}\label{Mon5:ListMonad}

 \begin{itemize}[<+->]
\item The \emph{list monad} consists of the following data:
 \begin{enumerate}
    \item the category $\HH$ of Haskell types and functions
    \item the list functor $[\_]:\HH\to\HH$, NB\footnote%
{We avoid the ambiguous notation $[f]$, which could also have type $[A\to B]$,
whereas the intended type here is $[A]\to [B]$.}
 $[\_](f)  =  map\, f$
    \item the natural transformation $\eta: id_\HH \To [\_]$, $\eta_A(a)= [a]$
    \item the natural transformation $\mu$, 
$\mu_A: [[A]] \to [A] $ defined by \emph{flattening}:
$\mu_A([]) = [],~\mu_A(l::ls) = l{+}\!{+}\mu_A(ls)$
 \end{enumerate}
%\item Exercise: figure out what $\mu_A$ does
\item The monad properties hold:
 \begin{enumerate}
    \item $\eta_{[A]};\mu_A = id_{[A]} = [\_](\eta_A);\mu_A$
    \item $[\_](\mu_A);\mu_A = \mu_{[A]};\mu_A$
 \end{enumerate}
\item Exercise: prove the above properties (compare with slide \ref{Mon5:PowSetMonad})
 \end{itemize}

 }

\frame
  {   
    \frametitle{The Maybe monad}\label{Mon5:ListMonad}

 \begin{itemize}[<+->]
\item The \href{https://wiki.haskell.org/All_About_Monads\#The_Maybe\_monad}%
{\color{blue}Maybe} monad is useful for partial functions
\item The \emph{Maybe monad} consists of the following data:
 \begin{enumerate}
    \item the category $\HH$ of Haskell types and functions
    \item the functor \ttt{ data Maybe t = Just t | Nothing}; %($t$ a type variable)
 \ttt{Maybe(f)(Just a) = Just (f a), Maybe(f)(\_) = Nothing}.
    \item the natural transformation $\eta: id_\HH \To \ttt{Maybe}$, $\eta_A(a)= \ttt{Just a}$
    \item the natural transformation $\mu: \ttt{Maybe;Maybe} \to \ttt{Maybe}$, 
$\mu_A(\ttt{Just(Just(a))})= \ttt{Just(a)}$,  $\mu_A(\ttt{\_})= \ttt{Nothing}$
 \end{enumerate}
%\item Exercise: figure out what $\mu_A$ does
\item The monad properties hold:
 \begin{enumerate}
    \item $\eta_\ttt{Maybe(A)};\mu_A = id_\ttt{Maybe(A)} =\ttt{Maybe}(\eta_A);\mu_A$
    \item $\ttt{Maybe}(\mu_A);\mu_A = \mu_\ttt{Maybe(A)};\mu_A$
 \end{enumerate}
\item Exercise: prove the above properties
 \end{itemize}

 }

\frame
  {   
    \frametitle{The Exception monad}\label{Mon5:ListMonad}

 \begin{itemize}[<+->]
\item The Exception monad empowers the
Maybe monad to signal not only \emph{that} something has gone wrong,
but also \emph{what}
\item Assume $E$ is some type whose values we call \emph{exceptions}
\item The \emph{ExcE monad} consists of the following data:
 \begin{enumerate}
    \item the category $\HH$ of Haskell types and functions
    \item the functor \ttt{data ExpE t = Inl t | InE E}, in CT: $ExpE(A)=A+E$;
%morphism%for $f:A\to B$
 \ttt{ExpE(f)(Inl a) = Inl(f a)},  \ttt{ExpE(f)(InE e) = (InE e)}, for $f:A\to B$
    \item the natural transformation $\eta$: \ttt{return a = Inl a}
    \item the natural transformation $\mu$, through $\bind$: 
$(\ttt{(Inl a)} \bind f) =  \ttt{(f a)}$,  $(\ttt{(InE e)} \bind f) =  \ttt{InE e}$
 \end{enumerate}
\item Exercise: prove the Haskel monad laws from slide \ref{Mon5:MonadHaskCtnd}.\\
Hint: for $m: ExpE(A)$ distinguish cases $Inl(a)$ and $InE(e)$.
 \end{itemize}

 }

\frame
  {   
    \frametitle{A monad for finite non-determinism}\label{Mon5:MonadNonDet}

 \begin{itemize}[<+->]
\item Non-determinism means that a computation can have zero or
more results (of the same type)
\item Finite non-determinism means that there are only finitely many results
\item The \emph{FinNonDet monad} is a variant of the power set monad,
slide \ref{Mon5:PowSetMonad}, where the functor is $\powfin$ on sets,
and extended to functions $f:A\to B$ by setting $\powfin(f)(X) = f(X)$,
and this {\color{red}image} is indeed in $\powfin(B)$ for $X\in\powfin(A)$.
\item Exercise: complete the definition of \emph{FinNonDet} and prove the monad laws
 \end{itemize}


 }

\frame
  {   
    \frametitle{Continuation Passing Style (CPS)}\label{Mon5:CPS}

 \begin{itemize}[<+->]
\item CPS is a style in which one does not define a function directly, but instead
defines how an extra function argument (the continuation of type $A\to R$) 
acts on the result of type $A$
\item The CPS form of a function $f: A\to B$ is a function $f_{\&_R} : A\to(B\to R)\to R$
such that $f_{\&_R} (a)(g) = g(f(a))$ for all $a\in A$, $g\in B\to R$ 
(we often omit subscript $R$ in $\&_R$)
\item For primitive functions $f$, $f_\&$ is defined as above, using $f$
\item Example: $(m+_\& n)(g) = g(m+n)$ for all $g:\nat\to R$
\item For more complicated functions, the CPS form
\begin{itemize}
    \item has arguments that are either variables or $\lambda$-expressions
    \item evaluates `inside-out' and makes the order of evaluation explicit
    \item reduces or avoids using a function stack
 \end{itemize}
\item CPS is more used in compilers than in actual programming
 \end{itemize}

 }

\frame
  {   
    \frametitle{CPS examples}\label{Mon5:CPS}

 \begin{itemize}[<+->]
\item The identity function in CPS would be $id_\& (a,c) = c(a)$
\item Consider the factorial $0! = 1,~(n+1)! = (n+1)*n!$; evaluation of 3! uses a stack:
$3! = 3*(2!) = 3*(2*(1!)) = 3*(2*(1*(0!))) = 3*(2*(1*1)) = 3*(2*1) = 3*2 = 6$
\item Tail recursive: $f(0,a) = a,~f(n+1,a) = f(n,a*(n+1))$ and $n! = f(n,1)$, stack-free!
Argument $a$ is called an \emph{accumulator}.
\item CPS factorial behaves a bit like the tail recursive variant
$0!_\&(c) = c(1),~(n+1)!_\&(c) = n!_\&(\lambda f_n. c((n+1)*f_n)$, now:\vspace*{2mm}
$3!_\&(c) = 2!_\&(\lambda f_2. c(3*f_2)) = 1!_\&(\lambda f_1. 
{\color{red}(\lambda f_2. c(3*f_2))(2*f_1)})$
$= 1!_\&(\lambda f_1. c(3*(2*f_1))) = 1!_\&(\lambda f_1. c(6*f_1)) =$
$= 0!_\&(\lambda f_0. 
{\color{red}(\lambda f_1. c(6*f_1))(1*f_0)}) = 0!_\&(\lambda f_0. c(6*(1*f_0))) $
$= (\lambda f_0. c(6*(1*f_0))) (1) = c(6*1*1) = c(6)$, stack-free!
\end{itemize}

 }

\frame
  {   
    \frametitle{The Continuation monad}\label{Mon5:MonadCont}

 \begin{itemize}[<+->]
\item In Haskell there is the 
\href{https://wiki.haskell.org/All_About_Monads\#The_Continuation\_monad}%
{\color{blue}Continuation} monad
\item The \emph{Continuation monad} consists of the following data:
 \begin{enumerate}
    \item the category $\Set$ (or $\HH$) and a set (or type) $R$
    \item the functor $C(A) = (A\to R)\to R$, $C(f) : C(A)\to C(B)$ defined by
$C(f)(g)(c) = g(f;c)$ for all $g: (A\to R)\to R, c: B\to R$ 
    \item the natural transformation $\eta$: $\ttt{return}\, a = \lambda c. c(a)$
    \item $\mu$ defined through $\bind$: %indirectly, by $\bind$:  
$(m \bind h) =  \lambda c. m(\lambda a. h(a)(c))$
 \end{enumerate}
\item Types: $m: (A\to R)\to R$, $h: A\to ((B\to R)\to R)$, 
$c: X\to R$ the $X$-continuations, for $X=A,B$.
\item Explanation: any $B$-continuation $c$ leads to an $A$-continuation 
$\lambda a. h(a)(c)$ using $h$, and then we use $m$ to get an $R$-value
\item Exercise: show that the Haskell monad laws hold
 \end{itemize}

 }

\frame
  {   
    \frametitle{State}\label{Mon5:State}

 \begin{itemize}[<+->]
\item An accumulator argument is an example of the use of state
\item Fibonacci: $f(0)=1, f(1)=1, f(n+2)=f(n+1)+f(n)$
\item Exponential: $f(n+2)$ computes $f(n)$ twice, etc.
\item Solution: $f(n)=g(n,1,1)$, $g(0,x,y)=y$, $g(1,x,y)=x$, $g(n+2,x,y)=g(n+1,x+y,x)$
\item Arguments $x,y$ encode a state of two natural numbers 
%a function $s:\set{x,y}\to\nat$
\item State-encoded-in-argument is impractical  for large states
\item Implicit machine state is not \emph{referentially transparent} (?)
\item A Fibonacci state is a pair $(x,y) : \nat^2$, the state transforma- tion
is $g(x,y)=(x+y,x)$, and $f(n) = \pi_1(g^n(1,0))$
\item The State monad makes it possible to separate the use of
state from the state-free parts of the program
 \end{itemize}

 }

\frame
  {   
    \frametitle{The State monad}\label{Mon5:MonadState}

 \begin{itemize}[<+->]
\item In Haskell there is the 
\href{https://wiki.haskell.org/All_About_Monads\#The_State\_monad}%
{\color{blue}State} monad
\item The \emph{State monad} consists of the following data:
 \begin{enumerate}
    \item the category $\Set$ (or $\HH$) and a set (or type) $S$
    \item the functor $St(A) = S \to (A\times S)$, $St(f) : St(A)\to St(B)$ defined by
$St(f)(\Kp{g,h})(s) = (f(g(s)),h(s))$ (NB $St$ for $St_S$)%for all $s\in S$ 
    \item the natural transformation $\eta$: $\ttt{return}\,a = \lambda s. (a,s)$
    \item $\mu$ defined through $\bind$:
$(\Kp{g,{\color{red}h}} \bind f ) =  \lambda s. f(g(s))({\color{red}h}(s))$
 \end{enumerate}
%\item Exercise: figure out what $\mu_A$ does
\item Types: $\Kp{g,h}: S \to (A\times S)$, $f: A\to (S \to (B\times S))$ 
\item Explanation: a monad value in $St_S(A)$ is a pair of functions  $\Kp{g,h}$
with $g:S\to A$ producing $A$-values and ${\color{red}h}:S\to S$ the state transformer.
Binding $f$ to $\Kp{g,{\color{red}h}}$ yields a monad value in $St_S(B)$, i.e.,
for every state $s$ we apply $f$ to the $A$-value $g(s)$ and 
the changed state ${\color{red}h}(s)$. The ${\color{red}h}$ is the magic!
\item Exercise: show that the Haskell monad laws hold
 \end{itemize}

 }

\frame
  {   
    \frametitle{Fibonacci with the State monad}\label{Mon5:FibState}

 \begin{itemize}[<+->]
\item Take $S=\nat^2$ and $A=\set{\bullet}$ ($A=()$ in Haskell) 
\item Define $f: A\to (S\to (A\times S))$ by $f(\bullet)(x,y) = (\bullet,(x+y,x))$
\item Define $put: S\to St(A)$ by $put(x,y) = \lambda\_.(\bullet,(x,y))$. Thus:
 \begin{itemize}
    \item $put(1,0)$ transforms any state to $(1,0)$ (we ignore $\bullet$)
    \item $put(1,0) \bind f$ transforms any state to $(1,1)$
    \item $put(1,0) \bind f \bind f$ transforms any state to $(2,1)$
    \item $put(1,0) \bind f \bind \cdots \bind f$  transforms any state to
a pair of successive Fibonacci numbers depending om \# of $f$'s
 \end{itemize}
\item Also: $(\eta_A(\bullet) \bind f \bind \cdots \bind f)(1,0) = (\bullet,(f_{n+1},f_n))$,
where $n$ is the number of $f$'s and $f_n$ the $n$-th Fibonacci number
\item Irony: this example is pure, it is pure state ...
\item Discussion of pro's and con's
%\item Exercise: program this in your favorite language with support for monads
 \end{itemize}
 }

\frame
  {   
    \frametitle{Fibonacci with the State monad in Haskell}\label{Mon5:FibStateHask}

 \begin{itemize}[<+->]
\item Haskell uses $()$ for $\set{\bullet}$ \emph{and} for ${\bullet}$
and has $put: S\to St_S(())$ defined by $put(s) = \lambda\_.((),s)$, changing any
current state to the argument $s$ of $put$, paired with (uninformative) value $()$
\item Haskell also has $get: St_S(S)$ defined by $get = \lambda s .(s,s)$,
returning the state as the value and not changing the state
\item \ttt{newtype State s a = State \{runState {:\!:} s->(a,s)\}}
\item In \href{https://github.com/mauget/fibonacci}{\color{blue}this implementation}
of Fibonacci in Haskell:
\begin{itemize}
    \item Fibonacci-states are triples of integers
    \item $S= \ttt{(Integer,Integer,Integer}), \,A = \ttt{Integer}$
    \item $\ttt{State(Integer,Integer,Integer})$ `is' the functor $St_S$ 
    \item $\ttt{fibsState} : St_S(\ttt{Integer})$ is a State monad computation
    \item $\ttt{evalState} : St_S(A)\to S\to A$ evaluates the result of state computation
    $m : St_S(A)$ with initial state $s$ to its $A$-value: \\
    \ttt{evalState m s = fst(runState m s)}
 %   \item 
 \end{itemize}

 \end{itemize}
 }

\frame
  {   
    \frametitle{Monads in other programming languages}\label{Mon5:InOtherPL}

 \begin{itemize}[<+->]

 \item  \href{https://curiosity-driven.org/monads-in-javascript}{\color{blue}JavaScript}

\item  \href{https://bartoszmilewski.com/2011/07/11/monads-in-c/}{\color{blue} C{+}{+}}

\item \href{https://docs.racket-lang.org/heresy/monad-do.html}
{\color{blue} Racket}

\item \href{https://dl.acm.org/doi/pdf/10.1145/1924421.1924436}
{\color{blue} LINQ} (= Language Independent Query)

 \end{itemize}
 }

\end{document}

\myurl{en.wikipedia.org/wiki/Ordered_pair}
 \begin{itemize}
    \item emulation halts because of the partiality of $\delta$;
    \item emulation halts because of "head left" with head at first cell;
    \item emulation halts because of reaching a halting state;
    \item the emulated TM goes on forever.
 \end{itemize}
